cas/theories/Tester.v
@@ -1,0 +1,206 @@
+From CAS Require Export
+     Observe.
+
+Definition exp_state:= list (var * (string + list string)).
+
+Definition fresh_var {T} (vs : list (var * T)) : var :=
+  S $ fold_left max (map fst vs) O.
+
+Definition fresh_value (s : exp_state) : exp_state * var :=
+  let x := fresh_var s in
+  (put x (inr []) s, x).
+
+Definition assert (x : var) (v : string) (s : exp_state) : string + exp_state :=
+  let ov := get x s in
+  let err := inl $ "Expect " ++ to_string ov
+        ++ ", but observed " ++ to_string v in
+  match ov with
+  | Some (inl v0) => if v =? v0 then inr s else err
+  | Some (inr vs) => if existsb (String.eqb v) vs
+                    then err else inr $ put x (inl v) s
+  | None          => inr $ put x (inl v) s
+  end.
+
+Definition assert_not (x : var) (v : string) (s : exp_state)
+  : string + exp_state :=
+  let ov := get x s in
+  let err := inl $ "Expect not " ++ to_string ov
+            ++ ", but observed " ++ to_string v in
+  match ov with
+  | Some (inl v0) => if v =? v0 then err else inr s
+  | Some (inr vs) => if existsb (String.eqb v) vs
+                    then inr s
+                    else inr $ put x (inr (v :: vs)) s
+  | None          => inr $ put x (inr [v]) s
+  end.
+
+Definition unify {T} (e : exp T) (v : T) (s : exp_state) : string + exp_state :=
+  match e in exp T return T -> exp_state -> string + exp_state with
+  | Exp__Const v0 =>
+    fun v s =>
+      if v = v0? then inr s
+      else inl $ "Expect " ++ to_string e ++ ", but observed " ++ to_string v
+  | Exp__Var x    => fun v s => assert x v s
+  | Exp__Match v0 (Exp__Var x) =>
+    fun b => if b then assert x v0 else assert_not x v0
+  | Exp__Match _ vx => fun _ _ => inl $ "Unexpected expression " ++ to_string vx
+  end v s.
+
+Variant testerE : Type -> Type :=
+  Tester__Recv : testerE (packetT id)
+| Tester__Send : server_state exp -> exp_state -> testerE (packetT id).
+
+Class Is__stE E `{failureE -< E} `{decideE -< E} `{testerE -< E}.
+Notation stE := (failureE +' decideE +' testerE).
+Instance stE_Is__stE : Is__stE stE. Defined.
+
+Definition instantiate_unify {E R} `{failureE -< E} (e : unifyE R)
+  : Monads.stateT exp_state (itree E) R :=
+  fun s =>
+    match e with
+    | Unify__Fresh =>
+      let (s', x) := fresh_value s in
+      Ret (s', Exp__Var x)
+    | Unify__Match bx b =>
+      match unify bx b s with
+      | inl err => throw $ "Unify match failed: " ++ err
+      | inr s'  => Ret (s', tt)
+      end
+    | Unify__Response rx r =>
+      match rx, r with
+      | Response__NotModified       , Response__NotModified
+      | Response__NoContent         , Response__NoContent
+      | Response__PreconditionFailed, Response__PreconditionFailed => ret (s, tt)
+      | Response__OK tx vx, Response__OK t v =>
+        match unify tx t s with
+        | inl err => throw $ "Unify tag failed: " ++ err
+        | inr s1  =>
+          match unify vx v s1 with
+          | inl err => throw $ "Unify value failed: " ++ err
+          | inr s2  => Ret (s2, tt)
+          end
+        end
+      | _, _ => throw $ "Expect response " ++ to_string rx
+                     ++ ", but observed " ++ to_string r
+      end
+    end.
+
+Definition instantiate_observe {E R} `{Is__stE E} (e : observeE R)
+  : Monads.stateT exp_state (itree E) R :=
+  fun s =>
+    match e with
+    | Observe__ToServer st => pkt <- embed Tester__Send st s;;
+                           Ret (s, pkt)
+    | Observe__FromServer  => pkt <- trigger Tester__Recv;;
+                           Ret (s, pkt)
+    end.
+
+Definition liftState {S A} {F : Type -> Type} `{Functor F} (aF : F A)
+  : Monads.stateT S F A :=
+  fun s : S => pair s <$> aF.
+
+Definition unifier' {E R} `{Is__stE E} (m : itree oE R)
+  : Monads.stateT exp_state (itree E) R :=
+  interp
+    (fun _ e =>
+       match e with
+       | (Throw err|) => fun s => throw err
+       | (|de|)       => liftState $ trigger de
+       | (||ue|)       => instantiate_unify ue
+       | (|||oe)      => instantiate_observe oe
+       end) m.
+
+Definition unifier {E R} `{Is__stE E} (m : itree oE R) : itree E R :=
+  snd <$> unifier' m [].
+
+CoFixpoint match_event {T R} (e0 : testerE R) (r : R) (m : itree stE T)
+  : itree stE T :=
+  match observe m with
+  | RetF x  => Ret x
+  | TauF m' => Tau (match_event e0 r m')
+  | VisF e k =>
+    match e with
+    | (||oe) =>
+      match oe in testerE Y, e0 in testerE R return (Y -> _) -> R -> _ with
+      | Tester__Send _ _, Tester__Send _ _
+      | Tester__Recv    , Tester__Recv => id
+      | _, _ => fun _ _ => throw "Unexpected event"
+      end k r
+    | _ => vis e (match_event e0 r ∘ k)
+    end
+  end.
+
+Definition match_observe {T R} (e : testerE T) (r : T) (l : list (itree stE R))
+  : list (itree stE R) := map (match_event e r) l.
+
+Variant clientE : Type -> Type :=
+| Client__Recv : clientE (option (packetT id))
+| Client__Send : server_state exp -> exp_state ->
+               clientE (option (packetT id)).
+
+Class Is__tE E `{failureE -< E} `{nondetE -< E} `{clientE -< E}.
+Notation tE := (failureE +' nondetE +' clientE).
+Instance tE_Is__tE : Is__tE tE. Defined.
+
+CoFixpoint backtrack' {E R} `{Is__tE E} (others : list (itree stE R))
+           (m : itree stE R) : itree E R :=
+  match observe m with
+  | RetF r => Ret r
+  | TauF m' => Tau (backtrack' others m')
+  | VisF e k =>
+    let catch (err : string) : itree E R :=
+        match others with
+        | [] => throw err
+        | other :: others' =>
+          (* embed Log ("Retry upon " ++ err);; *)
+          Tau (backtrack' others' other)
+        end in
+    match e with
+    | (Throw err|) => catch err
+    | (|de|) =>
+      match de in decideE Y return (Y -> _) -> _ with
+      | Decide => fun k => b <- trigger Or;;
+                       Tau (backtrack' (k (negb b) :: others) (k b))
+      end k
+    | (||te) =>
+      match te in testerE Y return (Y -> _) -> _ with
+      | Tester__Send st es =>
+        fun k => op1 <- trigger Client__Recv;;
+              match op1 with
+              | Some p1 =>
+                match match_observe Tester__Recv p1 others with
+                | [] => throw "Unexpected receive from server"
+                | other :: others' =>
+                  Tau (backtrack' others' other)
+                end
+              | None =>
+                opkt <- embed Client__Send st es;;
+                match opkt with
+                | Some pkt =>
+                  Tau (backtrack' (match_observe (Tester__Send st es)
+                                                 pkt others) (k pkt))
+                | None => catch "Not ready to send"
+                end
+              end
+      | Tester__Recv =>
+        fun k => opkt <- embed Client__Recv;;
+              match opkt with
+              | Some pkt =>
+                Tau (backtrack' (match_observe Tester__Recv pkt others) (k pkt))
+              | None =>
+                match others with
+                | [] =>
+                  Tau (backtrack' [] m)
+                | other :: others' =>
+                  Tau (backtrack' (others' ++ [m]) other)
+                end
+              end
+      end k
+    end
+  end.
+
+Definition backtrack {E R} `{Is__tE E} : itree stE R -> itree E R :=
+  backtrack' [].
+
+Definition tester {E R} `{Is__tE E} : itree oE R -> itree E R :=
+  backtrack ∘ unifier.
